code/chacha20poly1305/Hacl.Impl.Chacha20Poly1305.PolyCore.fst
@@ -1,0 +1,28 @@
+module Hacl.Impl.Chacha20Poly1305.PolyCore
+
+module ST = FStar.HyperStack.ST
+open FStar.HyperStack
+open FStar.HyperStack.All
+open Lib.IntTypes
+open Lib.Buffer
+open Lib.ByteBuffer
+open Lib.ByteSequence
+module Seq = Lib.Sequence
+open FStar.Mul
+
+module SpecPoly = Spec.Poly1305
+module Spec = Spec.Chacha20Poly1305
+module Poly = Hacl.Impl.Poly1305
+open Hacl.Impl.Poly1305.Fields
+
+let same_ctx_same_r_acc #s ctx h0 h1 = admit()
+
+let poly1305_padded #s ctx len text tmp = admit()
+
+let poly1305_init #s ctx k =
+//  Poly.poly1305_init ctx k;
+  admit()
+
+let update1 #s ctx len text = admit()
+
+let finish #s ctx k out = admit()
