code/chacha20poly1305/Hacl.Impl.Chacha20Poly1305.PolyCore.fsti
@@ -1,0 +1,91 @@
+module Hacl.Impl.Chacha20Poly1305.PolyCore
+
+module ST = FStar.HyperStack.ST
+open FStar.HyperStack
+open FStar.HyperStack.All
+open Lib.IntTypes
+open Lib.Buffer
+open Lib.ByteBuffer
+open Lib.ByteSequence
+module Seq = Lib.Sequence
+open FStar.Mul
+
+module SpecPoly = Spec.Poly1305
+module Spec = Spec.Chacha20Poly1305
+module Poly = Hacl.Impl.Poly1305
+open Hacl.Impl.Poly1305.Fields
+
+val same_ctx_same_r_acc:
+  #s:field_spec ->
+  ctx:Poly.poly1305_ctx s ->
+  h0:mem ->
+  h1:mem ->
+  Lemma
+    (requires Seq.equal (as_seq h0 ctx) (as_seq h1 ctx))
+    (ensures 
+      Seq.index (Poly.as_get_acc h0 ctx) 0 == Seq.index (Poly.as_get_acc h1 ctx) 0 /\
+      Seq.index (Poly.as_get_r h0 ctx) 0 == Seq.index (Poly.as_get_r h1 ctx) 0
+    )
+
+val poly1305_padded:
+  #s:field_spec ->
+  ctx:Poly.poly1305_ctx s ->
+  len:size_t ->
+  text:lbuffer uint8 len ->
+  tmp:lbuffer uint8 16ul ->
+  Stack unit
+    (requires fun h -> live h ctx /\ live h text /\ live h tmp)
+    (ensures fun h0 _ h1 -> 
+      modifies (loc tmp |+| loc ctx) h0 h1 /\
+      // Additional framing for r_elem
+      Seq.index (Poly.as_get_r h0 ctx) 0 == Seq.index (Poly.as_get_r h1 ctx) 0 /\
+      // Functional spec
+      Seq.index (Poly.as_get_acc h1 ctx) 0 == 
+      Spec.poly1305_padded 
+        (Seq.index (Poly.as_get_r h0 ctx) 0)
+        (v len)
+        (as_seq h0 text)
+        (as_seq h0 tmp)
+        (Seq.index (Poly.as_get_acc h0 ctx) 0)
+        )
+
+val poly1305_init:
+  #s:field_spec ->
+  ctx:Poly.poly1305_ctx s ->
+  k:lbuffer uint8 32ul ->
+  Stack unit
+    (requires fun h -> live h ctx /\ live h k)
+    (ensures fun h0 _ h1 -> modifies (loc ctx) h0 h1 /\
+      (let acc, r = SpecPoly.poly1305_init (as_seq h0 k) in
+      acc == Seq.index (Poly.as_get_acc h1 ctx) 0 /\
+      r == Seq.index (Poly.as_get_r h1 ctx) 0))
+
+val update1:
+  #s:field_spec ->
+  ctx:Poly.poly1305_ctx s ->
+  len:size_t{v len <= 16} ->
+  text:lbuffer uint8 len ->
+  Stack unit
+    (requires fun h -> live h ctx /\ live h text)
+    (ensures fun h0 _ h1 -> 
+      modifies (loc ctx) h0 h1 /\
+      // Additional framing for r_elem
+      Seq.index (Poly.as_get_r h0 ctx) 0 == Seq.index (Poly.as_get_r h1 ctx) 0 /\    
+      // Functional spec
+      Seq.index (Poly.as_get_acc h1 ctx) 0 == 
+      SpecPoly.update1
+        (Seq.index (Poly.as_get_r h0 ctx) 0)
+        (v len)
+        (as_seq h0 text)
+        (Seq.index (Poly.as_get_acc h0 ctx) 0)
+        )
+
+val finish:
+  #s:field_spec ->
+  ctx:Poly.poly1305_ctx s ->
+  k:lbuffer uint8 32ul -> // key
+  out:lbuffer uint8 16ul -> // output: tag
+  Stack unit
+    (requires fun h -> live h ctx /\ live h k /\ live h out)
+    (ensures fun h0 _ h1 -> modifies (loc out) h0 h1 /\
+      as_seq h1 out == SpecPoly.finish (as_seq h0 k) (Seq.index (Poly.as_get_acc h0 ctx) 0))
