code/chacha20poly1305/Hacl.Spec.Poly1305.Equiv.fst
@@ -1,0 +1,20 @@
+module Hacl.Spec.Poly1305.Equiv
+
+open FStar.Mul
+open Lib.IntTypes
+open Lib.Sequence
+open Lib.ByteSequence
+open Lib.IntVector
+
+module Poly = Spec.Poly1305
+module PolyVec = Hacl.Spec.Poly1305.Vec
+
+let update1_equiv (r:Poly.felem) (len:size_nat{len <= Poly.size_block}) (b:lbytes len) (acc:Poly.felem) 
+  : Lemma (Poly.update1 r len b acc = PolyVec.update1 r len b acc)
+  = admit()
+
+// let poly_equiv (text:bytes) (acc:Poly.felem) (r:Poly.felem)
+//   : Lemma (Poly.poly text acc r == PolyVec.poly #1 text (PolyVec.from_elem acc) (PolyVec.from_elem r)
+//   = admit()
+
+
